cfrontend/BeePL_Csyntax.v
@@ -1,90 +1,12 @@
 Require Import String ZArith Coq.FSets.FMapAVL Coq.Structures.OrderedTypeEx Coq.Strings.BinaryString.
 Require Import Coq.FSets.FSetProperties Coq.FSets.FMapFacts FMaps FSetAVL Nat PeanoNat Coq.Lists.List.
 Require Import Coq.Arith.EqNat Coq.ZArith.Int Integers AST Maps Ctypes Coqlib.
-Require Import BeePL_aux BeePL Csyntax Errors.
+Require Import BeePL_aux BeePL BeeTypes Csyntax Errors.
 
 Local Open Scope string_scope.
 Local Open Scope error_monad_scope.
 
-(****** Translation from BeePL to Csyntax ******)
-
-Section translate_types.
-
-Variable transBeePL_type : BeeTypes.type -> res Ctypes.type.
-
-(* Translates a list of BeePL types to list of Clight types *) 
-Fixpoint transBeePL_types (ts : list BeeTypes.type) : res Ctypes.typelist :=
-match ts with 
-| nil => OK Tnil
-| t :: ts => do ct <- (transBeePL_type t);
-             do cts <- (transBeePL_types ts);
-             OK (Tcons ct cts)
-end.
-
-End translate_types.
-
-Fixpoint typelist_list_type (ts : Ctypes.typelist) : list type :=
-match ts with
-| Tnil => nil
-| Tcons t ts => t :: typelist_list_type ts
-end. 
-
-Definition transBeePL_isize_cisize (sz : BeeTypes.intsize) : intsize :=
-match sz with 
-| BeeTypes.I8 => I8
-| BeeTypes.I16 => I16
-| BeeTypes.I32 => I32
-end.
-
-Definition transBeePL_sign_csign (s : BeeTypes.signedness) : signedness :=
-match s with 
-| BeeTypes.Signed => Signed
-| BeeTypes.Unsigned => Unsigned
-end.
-
-Definition compute_align (i : BeeTypes.intsize) : N :=
-match i with 
-| BeeTypes.I8 => 1%N
-| BeeTypes.I16 => 2%N
-| BeeTypes.I32 => 4%N
-end.
-
-(* Translation of BeePL types to Clight Types *) 
-Fixpoint transBeePL_type (t : BeeTypes.type) : res Ctypes.type :=
-match t with 
-| BeeTypes.Ptype (BeeTypes.Tunit) => OK (Tint I8 Unsigned {| attr_volatile := false; attr_alignas := Some 1%N |}) (* Fix me *)
-| BeeTypes.Ptype (BeeTypes.Tint sz s) => OK (Tint (transBeePL_isize_cisize sz) (transBeePL_sign_csign s)
-                                              {| attr_volatile := false; attr_alignas := Some (compute_align sz) |})
-| BeeTypes.Ptype (BeeTypes.Tbool) => OK (Tint I8 Unsigned {| attr_volatile := false; attr_alignas := Some 1%N |}) 
-| BeeTypes.Reftype h b => match b with 
-                          | BeeTypes.Bprim (BeeTypes.Tunit) => OK (Tpointer Tvoid {| attr_volatile := false; attr_alignas := Some 1%N |})
-                          | BeeTypes.Bprim (BeeTypes.Tint sz s) => OK (Tpointer (Tint (transBeePL_isize_cisize sz) (transBeePL_sign_csign s)
-                                                                             {| attr_volatile := false; attr_alignas := Some (compute_align sz) |})
-                                                              {| attr_volatile := false; attr_alignas := Some 8%N |})
-                          | BeeTypes.Bprim (BeeTypes.Tbool) => OK (Tpointer (Tint I8 Unsigned {| attr_volatile := false; 
-                                                                                             attr_alignas := Some 1%N |}) 
-                                                                   {| attr_volatile := false; attr_alignas := Some 8%N |})
-                          end
-| BeeTypes.Ftype ts ef t => do ats <- (transBeePL_types transBeePL_type ts);
-                            do rt <- (transBeePL_type t);
-                            OK (Tfunction ats rt {| cc_vararg := Some (Z.of_nat(length(ts))); cc_unproto := false; cc_structret := false |})  
-end.
-
-Definition bool_to_int (b : bool) : int :=
-match b with 
-| true => (Int.repr 1)
-| false => (Int.repr 0)
-end.
-
-(* Translates BeePL values to C values *)
-Definition transBeePL_value_cvalue (v : BeePL_mem.value) : Values.val :=
-match v with 
-| BeePL_mem.Vunit => Values.Vint (Int.repr 0) (* Fix me *)
-| BeePL_mem.Vint i => Values.Vint i
-| BeePL_mem.Vbool b => Values.Vint (bool_to_int b)
-| BeePL_mem.Vloc p => Values.Vptr p.(BeePL_mem.lname) (Ptrofs.of_ints (Int.repr 0))
-end.
-
+(**** BeePL Compiler *****)
 Section transBeePL_exprs.
 
 Variables transBeePL_expr_expr : BeePL.expr -> res Csyntax.expr.
@@ -100,45 +22,21 @@ end.
 
 End transBeePL_exprs.
 
-Definition transBeePL_uop_uop (uop : BeePL.uop) : Cop.unary_operation :=
-match uop with 
-| Notbool => Cop.Onotbool 
-| Notint => Cop.Onotint
-| Neg => Cop.Oneg
-end.
-
-Definition transBeePL_bop_bop (bop : BeePL.bop) : Cop.binary_operation :=
-match bop with 
-| Plus => Cop.Oadd
-| Minus => Cop.Osub
-| Mult => Cop.Omul
-| Div => Cop.Odiv
-| And => Cop.Oand
-| Or => Cop.Oor
-| Xor => Cop.Oxor
-| Shl => Cop.Oshl
-| Shr => Cop.Oshr
-| Eq => Cop.Oeq
-| Neq => Cop.One
-| Lt => Cop.Olt
-| Lte => Cop.Ole
-| Gt => Cop.Ogt
-| Gte => Cop.Oge
-end.
-
 Fixpoint exprlist_list_expr (es: Csyntax.exprlist) : list expr :=
 match es with 
 | Enil => nil 
 | Econs e1 es => (e1 :: exprlist_list_expr es)
 end.
 
+Definition default_expr := (Eval (Values.Vundef) Tvoid).
+
 Fixpoint transBeePL_expr_expr (e : BeePL.expr) : res Csyntax.expr := 
 match e with 
-| Var x => do xt <- (transBeePL_type (x.(BeePL_mem.vtype)));
-           OK (Evar x.(BeePL_mem.vname) xt)
+| Var x => do xt <- (transBeePL_type (vtype x));
+           OK (Evar (vname x) xt)
 | Const c t => match c with 
                | ConsInt i => do it <- (transBeePL_type t); OK (Eval (Values.Vint i) it)
-               | ConsBool b => do bt <- (transBeePL_type t); OK (Eval (Values.Vint (bool_to_int b)) bt)
+               | ConsLong i => do it <- (transBeePL_type t); OK (Eval (Values.Vlong i) it)
                | ConsUnit => do ut <- (transBeePL_type t); OK (Eval (Values.Vint (Int.repr 0)) ut) 
                end
 | App r e es t => do ce <- (transBeePL_expr_expr e); 
@@ -148,42 +46,28 @@ match e with
 | Prim b es t => match b with 
                  | Ref => do ces <- (transBeePL_expr_exprs transBeePL_expr_expr es);
                           do ct <- (transBeePL_type t);
-                          OK (Eaddrof (hd (Eval (Values.Vint (Int.repr 0))
-                                        (Tint I32 Signed {| attr_volatile := false; attr_alignas := Some 4%N |}))
-                                      (exprlist_list_expr ces)) 
+                          OK (Eaddrof (hd default_expr (exprlist_list_expr ces)) 
                               ct) 
                  | Deref => do ces <- (transBeePL_expr_exprs transBeePL_expr_expr es);
                             do ct <- (transBeePL_type t);
-                            OK (Ederef (hd  (Eval (Values.Vint (Int.repr 0))
-                                        (Tint I32 Signed {| attr_volatile := false; attr_alignas := Some 4%N |}))
-                                       (exprlist_list_expr ces)) 
+                            OK (Ederef (hd default_expr (exprlist_list_expr ces)) 
                                 ct)   
                  | Massgn => do ces <- (transBeePL_expr_exprs transBeePL_expr_expr es);
                              do ct <- (transBeePL_type t);
-                             OK (Eassign (hd  (Eval (Values.Vint (Int.repr 0))
-                                         (Tint I32 Signed {| attr_volatile := false; attr_alignas := Some 4%N |}))
-                                         (exprlist_list_expr ces))
-                                    (hd  (Eval (Values.Vint (Int.repr 0))
-                                       (Tint I32 Signed {| attr_volatile := false; attr_alignas := Some 4%N |}))
-                                     (tl (exprlist_list_expr ces)))
+                             OK (Eassign (hd default_expr (exprlist_list_expr ces))
+                                    (hd default_expr (tl (exprlist_list_expr ces)))
                                  ct)
                  | Run h => OK (Eval (Values.Vundef) Tvoid) (* Fix me *)
                  | Uop o => do ces <- (transBeePL_expr_exprs transBeePL_expr_expr es);
                             do ct <- (transBeePL_type t);
-                            OK (Eunop (transBeePL_uop_uop o) 
-                                (hd  (Eval (Values.Vint (Int.repr 0))
-                                       (Tint I32 Signed {| attr_volatile := false; attr_alignas := Some 4%N |}))
-                                (exprlist_list_expr ces)) 
+                            OK (Eunop o
+                                (hd default_expr (exprlist_list_expr ces)) 
                                 ct)
                  | Bop o => do ces <- (transBeePL_expr_exprs transBeePL_expr_expr es);
                             do ct <- (transBeePL_type t);
-                            OK (Ebinop (transBeePL_bop_bop o) 
-                                  (hd  (Eval (Values.Vint (Int.repr 0))
-                                       (Tint I32 Signed {| attr_volatile := false; attr_alignas := Some 4%N |}))
-                                   (exprlist_list_expr ces)) 
-                                  (hd  (Eval (Values.Vint (Int.repr 0))
-                                       (Tint I32 Signed {| attr_volatile := false; attr_alignas := Some 4%N |}))
-                                    (tl (exprlist_list_expr ces)))
+                            OK (Ebinop o
+                                  (hd default_expr (exprlist_list_expr ces)) 
+                                  (hd default_expr (tl (exprlist_list_expr ces)))
                                 ct)
                  end 
 | Bind x t e e' t' => do ct <- (transBeePL_type t);
@@ -196,8 +80,8 @@ match e with
                      do ce'' <- (transBeePL_expr_expr e'');
                      do ct <- (transBeePL_type t);
                      OK (Econdition ce ce' ce'' ct)  
-| Addr l => do ct <- (transBeePL_type l.(BeePL_mem.ltype));
-            OK (Eval (Values.Vptr l.(BeePL_mem.lname) (Ptrofs.of_ints (Int.repr 0))) ct)
+| Addr l => do ct <- (transBeePL_type (ltype l));
+            OK (Eval (Values.Vptr l.(lname) (Ptrofs.of_ints (Int.repr 0))) ct)
 | Hexpr h e t => OK (Eval (Values.Vundef) Tvoid) (* FIX ME *)
 end.
 
@@ -211,12 +95,12 @@ end.
 
 Definition transBeePL_expr_st (e : BeePL.expr) : res Csyntax.statement :=
 match e with 
-| Var x => do ct <- (transBeePL_type x.(BeePL_mem.vtype));
-           OK (Sreturn (Some (Evalof (Evar x.(BeePL_mem.vname) ct) ct)))
+| Var x => do ct <- (transBeePL_type x.(vtype));
+           OK (Sreturn (Some (Evalof (Evar x.(vname) ct) ct)))
 | Const c t => do ct <- (transBeePL_type t);
                OK (Sreturn (Some (Evalof (match c with 
                                       | ConsInt i => Eval (Values.Vint i) ct
-                                      | ConsBool b => Eval (Values.Vint (bool_to_int b)) ct
+                                      | ConsLong i => Eval (Values.Vlong i) ct
                                       | ConsUnit => Eval (Values.Vint (Int.repr 0)) ct
                                       end) ct)))
 | App r e es t => do ce <- (transBeePL_expr_expr e);
@@ -226,42 +110,28 @@ match e with
 | Prim b es t => match b with 
                  | Ref => do ces <- (transBeePL_expr_exprs transBeePL_expr_expr es);
                           do ct <- (transBeePL_type t);
-                          OK (Sdo (Eaddrof (hd  (Eval (Values.Vint (Int.repr 0))
-                                        (Tint I32 Signed {| attr_volatile := false; attr_alignas := Some 4%N |}))
-                                        (exprlist_list_expr ces)) 
+                          OK (Sdo (Eaddrof (hd default_expr (exprlist_list_expr ces)) 
                                    ct))   
                  | Deref => do ces <- (transBeePL_expr_exprs transBeePL_expr_expr es);
                             do ct <- (transBeePL_type t);
-                            OK (Sdo (Ederef (hd  (Eval (Values.Vint (Int.repr 0))
-                                        (Tint I32 Signed {| attr_volatile := false; attr_alignas := Some 4%N |}))
-                                         (exprlist_list_expr ces)) 
+                            OK (Sdo (Ederef (hd default_expr (exprlist_list_expr ces)) 
                                      ct))   
                  | Massgn => do ces <- (transBeePL_expr_exprs transBeePL_expr_expr es);
                              do ct <- (transBeePL_type t);
-                             OK (Sdo (Eassign (hd  (Eval (Values.Vint (Int.repr 0))
-                                               (Tint I32 Signed {| attr_volatile := false; attr_alignas := Some 4%N |}))
-                                               (exprlist_list_expr ces))
-                                              (hd  (Eval (Values.Vint (Int.repr 0))
-                                               (Tint I32 Signed {| attr_volatile := false; attr_alignas := Some 4%N |}))
-                                               (tl (exprlist_list_expr ces)))
+                             OK (Sdo (Eassign (hd default_expr (exprlist_list_expr ces))
+                                              (hd default_expr (tl (exprlist_list_expr ces)))
                                       ct)) 
                  | Run h => OK (Sdo (Eval (Values.Vundef) Tvoid)) (* Fix me *)
                  | Uop o => do ces <- (transBeePL_expr_exprs transBeePL_expr_expr es);
                             do ct <- (transBeePL_type t); 
-                            OK (Sdo (Eunop (transBeePL_uop_uop o) 
-                                     (hd (Eval (Values.Vint (Int.repr 0))
-                                       (Tint I32 Signed {| attr_volatile := false; attr_alignas := Some 4%N |}))
-                                      (exprlist_list_expr ces)) 
+                            OK (Sdo (Eunop o 
+                                     (hd default_expr (exprlist_list_expr ces)) 
                                      ct)) 
                  | Bop o => do ces <- (transBeePL_expr_exprs transBeePL_expr_expr es);
                             do ct <- (transBeePL_type t);
-                            OK (Sdo (Ebinop (transBeePL_bop_bop o) 
-                                     (hd (Eval (Values.Vint (Int.repr 0))
-                                         (Tint I32 Signed {| attr_volatile := false; attr_alignas := Some 4%N |}))
-                                        (exprlist_list_expr ces)) 
-                                     (hd (Eval (Values.Vint (Int.repr 0))
-                                         (Tint I32 Signed {| attr_volatile := false; attr_alignas := Some 4%N |}))
-                                      (tl (exprlist_list_expr ces)))
+                            OK (Sdo (Ebinop o 
+                                     (hd default_expr (exprlist_list_expr ces)) 
+                                     (hd default_expr (tl (exprlist_list_expr ces)))
                                      ct))
                  end 
 | Bind x t e e' t' => match e' with 
@@ -296,8 +166,8 @@ match e with
                                                         then OK (Sifthenelse ce (Sdo ce') (Sreturn (Some (Evalof ce'' ct'))))
                                                         else OK (Sifthenelse ce (Sdo ce') (Sdo ce''))
                       
-| Addr l => do ct <- (transBeePL_type l.(BeePL_mem.ltype)); 
-            OK (Sdo (Eval (Values.Vptr l.(BeePL_mem.lname) (Ptrofs.of_ints (Int.repr 0))) ct))
+| Addr l => do ct <- (transBeePL_type l.(ltype)); 
+            OK (Sdo (Eval (Values.Vptr l.(lname) (Ptrofs.of_ints (Int.repr 0))) ct))
 | Hexpr h e t => OK (Sdo (Eval (Values.Vundef) Tvoid)) (* FIX ME *)
 end.
 
@@ -308,14 +178,14 @@ Definition default_cc (fd : fun_decl) : calling_convention :=
 (* For now we have only internal functions: later change it to include the case of external function *)
 Definition BeePLfd_function (fd : fun_decl) : res (Ctypes.fundef function) :=
 do crt <- transBeePL_type (fd.(rtype));
-do pt <- (transBeePL_types transBeePL_type (unzip2 (BeePL_mem.extract_list_rvtypes (fd.(args)))));
-do vt <- (transBeePL_types transBeePL_type (unzip2 (BeePL_mem.extract_list_rvtypes (fd.(lvars)))));
+do pt <- (transBeePL_types transBeePL_type (unzip2 (extract_list_rvtypes (fd.(args)))));
+do vt <- (transBeePL_types transBeePL_type (unzip2 (extract_list_rvtypes (fd.(lvars)))));
 do fbody <- transBeePL_expr_st (fd.(body));
 OK (Internal {| fn_return := crt; 
                 fn_callconv := default_cc(fd); 
-                fn_params := zip (unzip1 (BeePL_mem.extract_list_rvtypes (fd.(args))))
+                fn_params := zip (unzip1 (extract_list_rvtypes (fd.(args))))
                                  (typelist_list_type pt);
-                fn_vars := zip (unzip1 (BeePL_mem.extract_list_rvtypes (fd.(lvars))))
+                fn_vars := zip (unzip1 (extract_list_rvtypes (fd.(lvars))))
                                (typelist_list_type vt);
                 fn_body :=  fbody|}).
 
@@ -324,7 +194,7 @@ Definition gconstant_init_data (g : BeePL.gconstant) : init_data :=
 match g with 
 | Gvalue c => match c with 
               | ConsInt i => Init_int32 i
-              | ConsBool b => Init_int8 (bool_to_int b)
+              | ConsLong i => Init_int64 i
               | ConsUnit => Init_int32 (Int.repr 0)
               end
 | Gloc p => Init_addrof p (Ptrofs.of_ints (Int.repr 0))
@@ -338,8 +208,8 @@ match gs with
 | g :: gs => gconstant_init_data g :: gconstants_init_datas gs
 end. 
 
-(* Translates BeePL global variable to C global variable *)
-Definition BeePLgd_gd (gv : globv) : res (globvar Ctypes.type)  :=
+(* Translates BeePL global variable to C global variable *) Print globv.
+Definition BeePLgd_gd (gv : glob_decl) : res (globvar Ctypes.type)  :=
 do gvt <- transBeePL_type (gv.(gtype));
 OK {| gvar_info := gvt; 
       gvar_init := gconstants_init_datas(gv.(gval)); 
@@ -347,16 +217,16 @@ OK {| gvar_info := gvt;
       gvar_volatile := false |}.
 
 (* Translates a BeePL declaration to C declaration *)
-Definition BeePLdecl_gdef (d : BeePL.decl) : res (globdef (Ctypes.fundef function) type) :=
+Definition BeePLdecl_gdef (d : BeePL.decl) : res (globdef (Ctypes.fundef function) Ctypes.type) :=
 match d with 
-| Fdecl fd => do cfd <- (BeePLfd_function fd); OK (Gfun cfd)
-| Gvdecl gd => do gv <- (BeePLgd_gd gd) ; OK (Gvar gv)
+| Fdecl (Fun fd) => do cfd <- (BeePLfd_function fd); OK (Gfun cfd)
+| Gvdecl (Glob gd) => do gv <- (BeePLgd_gd gd) ; OK (Gvar gv)
 (*| Tadecl ta => *) (* Fix me *)
 end.
 
 (* Translates a list of BeePL declarations to C declarations *)
 Fixpoint BeePLdecls_gdefs (ds : list BeePL.decl) : 
-res (list (globdef (Ctypes.fundef function) type)) :=
+res (list (globdef (Ctypes.fundef function) Ctypes.type)) :=
 match ds with 
 | nil => OK (nil)
 | d :: ds => do gd <- BeePLdecl_gdef d; 
@@ -371,11 +241,11 @@ unfold build_composite_env; simpl; reflexivity.
 Qed.
 
 (* Missing compositie information and list of public functions *) 
-Definition BeePL_compcert (m : BeePL.module) : res Csyntax.program :=
-do cfd <- (BeePLdecls_gdefs (unzip2 (fst(m)))); 
-OK {| prog_defs := (zip (unzip1 (fst (m))) cfd);
+Definition BeePL_compcert (m : BeePL.program) : res Csyntax.program :=
+do cfd <- (BeePLdecls_gdefs (unzip2 (m.(bprog_defs)))); 
+OK {| prog_defs := (zip (unzip1 (m.(bprog_defs))) cfd);
       prog_public := nil;
-      prog_main := snd(m);
+      prog_main := m.(bprog_main);
       prog_types := nil;
       prog_comp_env := (PTree.empty composite);
       prog_comp_env_eq := composite_default |}.
