cfrontend/BeeTypes.v
@@ -1,6 +1,9 @@
 Require Import String ZArith Coq.FSets.FMapAVL Coq.Structures.OrderedTypeEx.
-Require Import Coq.FSets.FSetProperties Coq.FSets.FMapFacts FMaps FSetAVL Nat PeanoNat.
+Require Import Coq.FSets.FSetProperties Coq.FSets.FMapFacts FMaps FSetAVL Nat PeanoNat Ctypes Errors.
 Require Import Coq.Arith.EqNat Coq.ZArith.Int Integers AST.
+
+Local Open Scope string_scope.
+Local Open Scope error_monad_scope.
 
 Inductive effect_label : Type :=
 | Panic : effect_label               (* exception effect *)
@@ -11,64 +14,25 @@ Inductive effect_label : Type :=
 
 Definition effect := list effect_label.  (* row of effects *)
 
-Inductive signedness : Type :=
-| Signed: signedness
-| Unsigned: signedness.
-
-Inductive intsize : Type :=
-| I8: intsize
-| I16: intsize
-| I32: intsize.
-
-Inductive primitive_type : Type :=
-| Tunit : primitive_type
-| Tint : intsize -> signedness -> primitive_type
-| Tbool : primitive_type.
-
-Inductive basic_type : Type :=  
-| Bprim : primitive_type -> basic_type.
-
 Inductive type : Type :=
-| Ptype : primitive_type -> type                          (* primitive types *)
-| Reftype : ident -> basic_type -> type                   (* reference type ref<h,int> *)
-| Ftype : list type -> effect -> type -> type             (* function/arrow type *).
+| Tunit : type
+| Tint : intsize -> signedness -> attr -> type
+| Tlong : signedness -> attr -> type               (* primitive types *)
+| Reftype : ident -> type -> attr -> type          (* reference type ref<h,int> *)
+| Ftype : list type -> effect -> type -> type       (* function/arrow type *).
 
-Definition sizeof_ptype (t : primitive_type) : Z :=
+Fixpoint sizeof_type (t : type) : Z :=
 match t with 
 | Tunit => 1
-| Tint I8 _ => 1
-| Tint I16 _ => 2
-| Tint I32 _ => 4
-| Tbool => 1
-end.
-
-Definition sizeof_btype (t : basic_type) : Z :=
-match t with 
-| Bprim t => sizeof_ptype t 
-end. 
-
-Definition sizeof_type (t : type) : Z :=
-match t with 
-| Ptype t => sizeof_ptype t 
-| Reftype h t => sizeof_btype t + 1 (* 1 taking for the h *)
+| Tint I8 _ _ => 1
+| Tint I16 _ _ => 2
+| Tint I32 _ _ => 4
+| Tint IBool _ _ => 1
+| Tlong _ _ => 8
+| Reftype h t _ => sizeof_type t + 1 (* 1 taking for the h *)
 | Ftype ts e t => 1
 end.
 
-(* Equality on types *)
-Definition eq_signedness (sg1 sg2 : signedness) : bool :=
-match sg1, sg2 with 
-| Signed, Signed => true 
-| Unsigned, Unsigned => true 
-| _, _ => false
-end.
-
-Definition eq_intsize (i1 i2: intsize) : bool :=
-match i1, i2 with 
-| I8, I8 => true 
-| I16, I16 => true 
-| I32, I32 => true 
-| _, _ => false
-end.
 
 Definition eq_effect_label (e1 e2 : effect_label) : bool :=
 match e1, e2 with 
@@ -87,32 +51,6 @@ match es1, es2 with
 | _, _ => false
 end.
 
-Definition eq_primitive_type (p1 p2 : primitive_type) : bool :=
-match p1, p2 with 
-| Tunit, Tunit => true 
-| Tint sz s, Tint sz' s'=> eq_intsize sz sz' && eq_signedness s s'
-| Tbool, Tbool => true
-| _, _ => false
-end.   
-
-Section Eq_basic_types.
-
-Variable eq_basic_type : basic_type -> basic_type -> bool.
-
-Fixpoint eq_basic_types (bs1 bs2 : list basic_type) : bool :=
-match bs1, bs2 with 
-| nil, nil => true 
-| x :: xs, x' :: xs' => eq_basic_type x x' && eq_basic_types xs xs'
-| _, _ => false
-end.
-
-End Eq_basic_types.
-
-Definition eq_basic_type (b1 b2 : basic_type) : bool :=
-match b1, b2 with 
-| Bprim p1, Bprim p2 => eq_primitive_type p1 p2
-end.
-
 Section Eq_types.
 
 Variable eq_type : type -> type -> bool.
@@ -126,15 +64,91 @@ end.
 
 End Eq_types.
 
-Fixpoint eq_type (t1 t2 : type) : bool :=
-match t1,t2 with 
-| Ptype b1, Ptype b2 => eq_primitive_type b1 b2
+Fixpoint eq_type (p1 p2 : type) : bool :=
+match p1, p2 with 
+| Tunit, Tunit => true 
+| Tint sz s a, Tint sz' s' a'=> if intsize_eq sz sz' 
+                                then if signedness_eq s s'
+                                     then if attr_eq a a'
+                                          then true 
+                                          else false
+                                     else false
+                                else false
+| Tlong s a, Tlong s' a' => if signedness_eq s s'
+                            then if attr_eq a a'
+                                 then true 
+                                 else false
+                            else false
 | Ftype ts1 e1 t1, Ftype ts2 e2 t2 => 
   eq_types eq_type ts1 ts2 && eq_effect e1 e2 && eq_type t1 t2
-| Reftype e1 b1, Reftype e2 b2 => (e1 =? e2)%positive && eq_basic_type b1 b2 
+| Reftype e1 b1 a1, Reftype e2 b2 a2 => if attr_eq a1 a2  
+                                        then (e1 =? e2)%positive && eq_type b1 b2
+                                        else false
 | _, _ => false
+end.   
+
+(** ** Access modes *)
+
+(** The [access_mode] function describes how a l-value of the given
+type must be accessed:
+- [By_value ch]: access by value, i.e. by loading from the address
+  of the l-value using the memory chunk [ch];
+- [By_reference]: access by reference, i.e. by just returning
+  the address of the l-value (used for arrays and functions);
+- [By_copy]: access is by reference, assignment is by copy
+  (used for [struct] and [union] types)
+- [By_nothing]: no access is possible, e.g. for the [void] type.
+*)
+
+Definition access_mode (t : type) : mode :=
+match t with 
+| Tunit => By_nothing
+| Tint I8 Signed _ => By_value Mint8signed
+| Tint I8 Unsigned _ => By_value Mint8unsigned
+| Tint I16 Signed _ => By_value Mint16signed
+| Tint I16 Unsigned _ => By_value Mint16unsigned
+| Tint I32 _ _ => By_value Mint32
+| Tint IBool _ _ => By_value Mbool
+| Tlong _ _ => By_value Mint64
+| Reftype h t _ => By_value Mptr
+| Ftype ts ef t => By_reference
 end.
 
+(****** Translation from BeePL types to Csyntax types ******)
+
+Section translate_types.
+
+Variable transBeePL_type : BeeTypes.type -> res Ctypes.type.
+
+(* Translates a list of BeePL types to list of Clight types *) 
+Fixpoint transBeePL_types (ts : list BeeTypes.type) : res Ctypes.typelist :=
+match ts with 
+| nil => OK Tnil
+| t :: ts => do ct <- (transBeePL_type t);
+             do cts <- (transBeePL_types ts);
+             OK (Tcons ct cts)
+end.
+
+End translate_types.
+
+Fixpoint typelist_list_type (ts : Ctypes.typelist) : list Ctypes.type :=
+match ts with
+| Tnil => nil
+| Tcons t ts => t :: typelist_list_type ts
+end. 
+
+(* Translation of BeePL types to Clight Types *)
+Fixpoint transBeePL_type (t : BeeTypes.type) : res Ctypes.type :=
+match t with 
+| Tunit => OK (Ctypes.Tint I8 Unsigned {| attr_volatile := false; attr_alignas := Some 1%N |}) (* Fix me *)
+| Tint sz s a => OK (Ctypes.Tint sz s a)
+| Tlong s a => OK (Ctypes.Tlong s a)
+| Reftype h t a => do ct <- transBeePL_type t;
+                 OK (Tpointer ct a)
+| BeeTypes.Ftype ts ef t => do ats <- (transBeePL_types transBeePL_type ts);
+                            do rt <- (transBeePL_type t);
+                            OK (Tfunction ats rt {| cc_vararg := Some (Z.of_nat(length(ts))); cc_unproto := false; cc_structret := false |})  
+end.
 
 (* Typing context *)
 Definition ty_context := list (ident * type).
